Add definitions for the stateful function signatures in Hacl.Streaming.Functor.fsti

code/streaming/Hacl.Streaming.Functor.fsti
@@ -226,12 +226,12 @@ val index_of_state:
   (fun h0 i' h1 -> h0 == h1 /\ i' == i))
 
 inline_for_extraction noextract
-val create_in:
-  #index: Type0 ->
-  c:block index ->
-  i:index ->
-  t:Type0 { t == c.state.s i } ->
-  t':Type0 { t' == optional_key i c.km c.key } ->
+let create_in_st
+  (#index: Type0)
+  (c:block index)
+  (i:index)
+  (t:Type0 { t == c.state.s i })
+  (t':Type0 { t' == optional_key i c.km c.key }) =
   k:c.key.s i ->
   r: HS.rid ->
   ST (state c i t t')
@@ -248,12 +248,21 @@ val create_in:
     B.(loc_includes (loc_region_only true r) (footprint c i h1 s))))
 
 inline_for_extraction noextract
-val alloca:
+val create_in:
   #index: Type0 ->
   c:block index ->
   i:index ->
   t:Type0 { t == c.state.s i } ->
   t':Type0 { t' == optional_key i c.km c.key } ->
+  create_in_st c i t t'
+
+inline_for_extraction noextract
+let alloca_st
+  (#index: Type0)
+  (c:block index)
+  (i:index)
+  (t:Type0 { t == c.state.s i })
+  (t':Type0 { t' == optional_key i c.km c.key }) =
   k:c.key.s i ->
   StackInline (state c i t t')
   (requires (fun h0 ->
@@ -266,15 +275,23 @@ val alloca:
     B.fresh_loc (footprint c i h1 s) h0 h1 /\
     B.(loc_includes (loc_region_only true (HS.get_tip h1)) (footprint c i h1 s))))
 
-/// Note: this is more like a "reinit" function so that clients can reuse the state.
 inline_for_extraction noextract
-val init:
-  #index:Type0 ->
+val alloca:
+  #index: Type0 ->
   c:block index ->
-  i:G.erased index -> (
-  let i = G.reveal i in
+  i:index ->
   t:Type0 { t == c.state.s i } ->
   t':Type0 { t' == optional_key i c.km c.key } ->
+  alloca_st #index c i t t'
+
+/// Note: this is more like a "reinit" function so that clients can reuse the state.
+inline_for_extraction noextract
+let init_st
+  (#index: Type0)
+  (c:block index)
+  (i:index)
+  (t:Type0 { t == c.state.s i })
+  (t':Type0 { t' == optional_key i c.km c.key }) =
   k:c.key.s i ->
   s:state c i t t' ->
   Stack unit
@@ -287,7 +304,17 @@ val init:
     seen c i h1 s == S.empty /\
     key c i h1 s == c.key.v i h0 k /\
     footprint c i h0 s == footprint c i h1 s /\
-    B.(modifies (footprint c i h0 s) h0 h1))))
+    B.(modifies (footprint c i h0 s) h0 h1)))
+
+inline_for_extraction noextract
+val init:
+  #index:Type0 ->
+  c:block index ->
+  i:G.erased index -> (
+  let i = G.reveal i in
+  t:Type0 { t == c.state.s i } ->
+  t':Type0 { t' == optional_key i c.km c.key } ->
+  init_st #index c i t t')
 
 unfold noextract
 let update_pre
@@ -322,6 +349,20 @@ let update_post
   key c i h1 s == key c i h0 s
 
 inline_for_extraction noextract
+let update_st
+  (#index: Type0)
+  (c:block index)
+  (i:index)
+  (t:Type0 { t == c.state.s i })
+  (t':Type0 { t' == optional_key i c.km c.key }) =
+  s:state c i t t' ->
+  data: B.buffer uint8 ->
+  len: UInt32.t ->
+  Stack unit
+    (requires fun h0 -> update_pre c i s data len h0)
+    (ensures fun h0 s' h1 -> update_post c i s data len h0 h1)
+
+inline_for_extraction noextract
 val update:
   #index:Type0 ->
   c:block index ->
@@ -329,12 +370,7 @@ val update:
   let i = G.reveal i in
   t:Type0 { t == c.state.s i } ->
   t':Type0 { t' == optional_key i c.km c.key } ->
-  s:state c i t t' ->
-  data: B.buffer uint8 ->
-  len: UInt32.t ->
-  Stack unit
-    (requires fun h0 -> update_pre c i s data len h0)
-    (ensures fun h0 s' h1 -> update_post c i s data len h0 h1))
+  update_st #index c i t t')
 
 inline_for_extraction noextract
 let finish_st
@@ -379,6 +415,21 @@ val mk_finish:
   finish_st c i t t'
 
 inline_for_extraction noextract
+let free_st
+  (#index: Type0)
+  (c:block index)
+  (i:index)
+  (t:Type0 { t == c.state.s i })
+  (t':Type0 { t' == optional_key i c.km c.key }) =
+  s:state c i t t' ->
+  ST unit
+  (requires fun h0 ->
+    invariant c i h0 s /\
+    freeable c i h0 s)
+  (ensures fun h0 _ h1 ->
+    B.modifies (footprint c i h0 s) h0 h1)
+
+inline_for_extraction noextract
 val free:
   #index:Type0 ->
   c:block index ->
@@ -386,10 +437,4 @@ val free:
   let i = G.reveal i in
   t:Type0 { t == c.state.s i } ->
   t':Type0 { t' == optional_key i c.km c.key } ->
-  s:state c i t t' ->
-  ST unit
-  (requires fun h0 ->
-    invariant c i h0 s /\
-    freeable c i h0 s)
-  (ensures fun h0 _ h1 ->
-    B.modifies (footprint c i h0 s) h0 h1))
+  free_st #index c i t t')
